README.md
@@ -4,10 +4,9 @@
 
 - [x] Prove the preservation of the functional transition
 - [x] Prove the progress of the functional transition
-- [ ] Prove the preservation of the temporal transition
-- [ ] Prove the progress of the temporal transition
+- [x] Prove the preservation of the temporal transition
+- [x] Prove the progress of the temporal transition
 - [x] Prove the safety property for the functional transition
-- [ ] Prove the safety property for the temporal transition
 
 ## Dependencies
 
